src/RqUpRed.v
@@ -11,6 +11,14 @@ Set Implicit Arguments.
 Open Scope list.
 Open Scope fmap.
 
+Ltac disc_rqUpMsgs :=
+  match goal with
+  | [H: RqUpMsgs _ _ _ |- _] =>
+    let cidx := fresh "cidx" in
+    let rqUp := fresh "rqUp" in
+    destruct H as [cidx [rqUp ?]]; dest
+  end.
+
 Ltac disc_rqToUpRule :=
   match goal with
   | [H: RqToUpRule _ _ _ |- _] =>
@@ -167,7 +175,7 @@ Section RqUpReduction.
 
   Ltac disc_rule_custom ::=
     try disc_footprints_ok;
-    try disc_msgs_in.
+    try disc_rqUpMsgs.
   
   Lemma rqUpMsgs_RqToUpRule:
     forall {oifc} (sys: System oifc) oidx (rule: Rule oifc)
@@ -305,7 +313,7 @@ Section RqUpReduction.
   Ltac disc_rule_custom ::=
     try disc_lock_conds;
     try disc_footprints_ok;
-    try disc_msgs_in;
+    try disc_rqUpMsgs;
     try disc_rqToUpRule.
 
   Lemma rqUp_lbl_commutes:
